src/spec/TLS13.StateMachine.fst
@@ -159,6 +159,14 @@ let lemma_advance_read_records_succ (s:conn_state) (n:nat)
   =
   ()
 
+let rec lemma_advance_read_records_after_one (s:conn_state) (n:nat)
+  : Lemma
+      (ensures advance_read_records (advance_read_record s) n == advance_read_records s (n + 1))
+          (decreases n)
+  =
+  if n = 0 then lemma_advance_read_records_one s
+  else lemma_advance_read_records_after_one s (n - 1)
+
 let rec lemma_advance_read_records_read_seq (s:conn_state) (n:nat)
   : Lemma
       (ensures (advance_read_records s n).read_state.R.seq == s.read_state.R.seq + n)
